% Exercise 2.1.4

\begin{itemize}
    \item[(a)] We begin by evaluating 
        \[
            t = \ln{\biggl\lvert\frac{\csc{x_0} + \cot{x_0}}{\csc{x} + \cot{x}}\biggr\rvert}
        \]
        with $x_0 = \pi / 4$ to find
        \begin{equation*}
            \begin{split}
                t &= \ln{\biggl\lvert\frac{\sqrt{2} + 1}{\csc{x} + \cot{x}}\biggr\rvert} \\
                  &= \ln{\biggl(\frac{1 + \sqrt{2}}{\csc{x} + \cot{x}}\biggr)}.
            \end{split}
        \end{equation*}
        Then we apply the function $e^z$ to both sides of to find
        \begin{equation*}
            \begin{split}
                e^t &= \frac{1 + \sqrt{2}}{\csc{x} + \cot{x}} \\
                    &= \frac{1 + \sqrt{2}}{\cot{(x/2)}} \\
                \Leftrightarrow \cot{(x/2)} &= \frac{1 + \sqrt{2}}{e^t} \\
                \Leftrightarrow \frac{1}{\tan{(x/2)}} &= \frac{1 + \sqrt{2}}{e^t} \\
                \Leftrightarrow \tan{(x/2)} &= \frac{e^t}{1 + \sqrt{2}} \\
                \Leftrightarrow \frac{x}{2} &= \tan^{-1}{\biggl(\frac{e^t}{1 + \sqrt{2}}\biggr)} \\
                \Leftrightarrow x &= 2\tan^{-1}{\biggl(\frac{e^t}{1 + \sqrt{2}}\biggr)}.
            \end{split}
        \end{equation*}
        Now, we have
        \[
            \lim_{t \rightarrow \infty} x(t) = \lim_{t \rightarrow \infty}
            \biggl[2\tan^{-1}{\biggl(\frac{e^t}{1 + \sqrt{2}}\biggr)}\biggr] = \pi,
        \]
        since $\lim_{t \rightarrow \infty}e^t = \infty$ and 
        $\lim_{t \rightarrow \infty}\tan^{-1}{t} = \pi$.
    \item[(b)] An analytic solution is given by performing the steps in (a) without 
        assuming $x_0 = \pi / 4$, so that we have
        \begin{equation*}
            \begin{split}
                x(t) &= 2\tan^{-1}{\biggl(\frac{e^t}{\csc{x_0} + \cot{x_0}}\biggr)} \\
                     &= 2\tan^{-1}{\biggl(\frac{e^t}{\cot{(x_0/2)}}\biggr)}.
            \end{split}
        \end{equation*}
\end{itemize}
